Attempt at using with_tactic for Steel VC generation

pulse/ulib/experimental/Steel.Effect.Atomic.fsti
@@ -66,7 +66,7 @@ let return_req (p:vprop) : req_t p = fun _ -> True
 /// and return leaves selectors of all resources in [p] unchanged
 unfold
 let return_ens (a:Type) (x:a) (p:a -> vprop) : ens_t (p x) a p =
-  fun h0 r h1 -> normal (r == x /\ frame_equalities (p x) h0 h1)
+  fun h0 r h1 -> r == x /\ frame_equalities (p x) h0 h1
 
 /// Monadic return combinator for the Steel effect. It is parametric in the postcondition
 /// The vprop precondition is annotated with the return_pre predicate to enable special handling,
@@ -92,14 +92,14 @@ let bind_req (#a:Type)
   (frame_f:vprop) (frame_g:a -> vprop)
   (_:squash (can_be_split_forall_dep pr (fun x -> post_f x `star` frame_f) (fun x -> pre_g x `star` frame_g x)))
 : req_t (pre_f `star` frame_f)
-= fun m0 -> normal (
+= fun m0 ->
   req_f (focus_rmem m0 pre_f) /\
   (forall (x:a) (h1:hmem (post_f x `star` frame_f)).
     (ens_f (focus_rmem m0 pre_f) x (focus_rmem (mk_rmem (post_f x `star` frame_f) h1) (post_f x)) /\
       frame_equalities frame_f (focus_rmem m0 frame_f) (focus_rmem (mk_rmem (post_f x `star` frame_f) h1) frame_f))
     ==> pr x /\
       (can_be_split_trans (post_f x `star` frame_f) (pre_g x `star` frame_g x) (pre_g x);
-      (req_g x) (focus_rmem (mk_rmem (post_f x `star` frame_f) h1) (pre_g x)))))
+      (req_g x) (focus_rmem (mk_rmem (post_f x `star` frame_f) h1) (pre_g x))))
 
 /// Logical postcondition for the composition (bind) of two Steel computations:
 /// The precondition of the first computation was satisfied in the initial state, and there
@@ -118,7 +118,7 @@ let bind_ens (#a:Type) (#b:Type)
   (_:squash (can_be_split_forall_dep pr (fun x -> post_f x `star` frame_f) (fun x -> pre_g x `star` frame_g x)))
   (_:squash (can_be_split_post (fun x y -> post_g x y `star` frame_g x) post))
 : ens_t (pre_f `star` frame_f) b post
-= fun m0 y m2 -> normal (
+= fun m0 y m2 ->
   req_f (focus_rmem m0 pre_f) /\
   (exists (x:a) (h1:hmem (post_f x `star` frame_f)).
     pr x /\
@@ -130,7 +130,7 @@ let bind_ens (#a:Type) (#b:Type)
     frame_equalities frame_f (focus_rmem m0 frame_f) (focus_rmem (mk_rmem (post_f x `star` frame_f) h1) frame_f) /\
     frame_equalities (frame_g x) (focus_rmem (mk_rmem (post_f x `star` frame_f) h1) (frame_g x)) (focus_rmem m2 (frame_g x)) /\
     ens_f (focus_rmem m0 pre_f) x (focus_rmem (mk_rmem (post_f x `star` frame_f) h1) (post_f x)) /\
-    (ens_g x) (focus_rmem (mk_rmem (post_f x `star` frame_f) h1) (pre_g x)) y (focus_rmem m2 (post_g x y)))))
+    (ens_g x) (focus_rmem (mk_rmem (post_f x `star` frame_f) h1) (pre_g x)) y (focus_rmem m2 (post_g x y))))
 
 /// Steel atomic effect combinator to compose two Steel atomic computations
 /// Separation logic VCs are squashed goals passed as implicits, annotated with the framing_implicit
@@ -175,10 +175,9 @@ let subcomp_pre (#a:Type)
   (_:squash (can_be_split pre_g pre_f))
   (_:squash (equiv_forall post_f post_g))
 : pure_pre
-= (forall (h0:hmem pre_g). normal (req_g (mk_rmem pre_g h0) ==> req_f (focus_rmem (mk_rmem pre_g h0)  pre_f))) /\
-  (forall (h0:hmem pre_g) (x:a) (h1:hmem (post_g x)). normal (
+= (forall (h0:hmem pre_g). req_g (mk_rmem pre_g h0) ==> req_f (focus_rmem (mk_rmem pre_g h0)  pre_f)) /\
+  (forall (h0:hmem pre_g) (x:a) (h1:hmem (post_g x)).
       ens_f (focus_rmem (mk_rmem pre_g h0) pre_f) x (focus_rmem (mk_rmem (post_g x) h1) (post_f x)) ==> ens_g (mk_rmem pre_g h0) x (mk_rmem (post_g x) h1)
-    )
   )
 
 /// Subtyping combinator for Steel atomic computations.
@@ -202,7 +201,7 @@ val subcomp (a:Type)
   (f:repr a framed_f opened_invariants o1 pre_f post_f req_f ens_f)
 : Pure (repr a framed_g opened_invariants o2 pre_g post_g req_g ens_g)
        (requires (o1 = Unobservable || o2 = Observable) /\
-         subcomp_pre req_f ens_f req_g ens_g p1 p2)
+         normal (subcomp_pre req_f ens_f req_g ens_g p1 p2))
        (ensures fun _ -> True)
 
 /// Logical precondition for the if_then_else combinator
@@ -213,10 +212,9 @@ let if_then_else_req
   (req_then:req_t pre_f) (req_else:req_t pre_g)
   (p:Type0)
 : req_t pre_f
-= fun h -> normal (
+= fun h ->
     (p ==> req_then (focus_rmem h pre_f)) /\
     ((~ p) ==> req_else (focus_rmem h pre_g))
-  )
 
 /// Logical postcondition for the if_then_else combinator
 unfold
@@ -227,10 +225,9 @@ let if_then_else_ens (#a:Type)
   (ens_then:ens_t pre_f a post_f) (ens_else:ens_t pre_g a post_g)
   (p:Type0)
 : ens_t pre_f a post_f
-= fun h0 x h1 -> normal (
+= fun h0 x h1 ->
     (p ==> ens_then (focus_rmem h0 pre_f) x (focus_rmem h1 (post_f x))) /\
     ((~ p) ==> ens_else (focus_rmem h0 pre_g) x (focus_rmem h1 (post_g x)))
-  )
 
 /// If_then_else combinator for Steel computations.
 /// The soundness of this combinator is automatically proven with respect to the subcomp
@@ -314,7 +311,7 @@ unfold
 let bind_pure_steel__req (#a:Type) (wp:pure_wp a)
   (#pre:pre_t) (req:a -> req_t pre)
 : req_t pre
-= fun m -> normal ((wp (fun x -> (req x) m) /\ as_requires wp))
+= fun m -> wp (fun x -> (req x) m) /\ as_requires wp
 
 /// Logical postcondition of a Pure and a SteelAtomic composition.
 /// There exists an intermediate value (the output of the Pure computation) such that
@@ -324,7 +321,7 @@ let bind_pure_steel__ens (#a:Type) (#b:Type)
   (wp:pure_wp a)
   (#pre:pre_t) (#post:post_t b) (ens:a -> ens_t pre b post)
 : ens_t pre b post
-= fun m0 r m1 -> normal ((as_requires wp /\ (exists (x:a). as_ensures wp x /\ ((ens x) m0 r m1))))
+= fun m0 r m1 -> as_requires wp /\ (exists (x:a). as_ensures wp x /\ ((ens x) m0 r m1))
 
 /// The composition combinator
 val bind_pure_steela_ (a:Type) (b:Type)
@@ -455,7 +452,7 @@ val get (#p:vprop) (#opened:inames) (_:unit) : SteelGhostF (erased (rmem p))
   opened
   p (fun _ -> p)
   (requires fun _ -> True)
-  (ensures fun h0 r h1 -> normal (frame_equalities p h0 h1 /\ frame_equalities p r h1))
+  (ensures fun h0 r h1 -> frame_equalities p h0 h1 /\ frame_equalities p r h1)
 
 /// Returning the current value of the selector of vprop [p], as long as [p] is in the context
 let gget (#opened:inames) (p: vprop) : SteelGhost (erased (t_of p))
